aarch64 refine: add armKSVMIDTable validity for CRefine
In ADT_C in CRefine we need to know that the VMID table is reversible,
which means it cannot contain any "Some 0" pointers.

Signed-off-by: Gerwin Klein <gerwin.klein@proofcraft.systems>

proof/refine/AARCH64/Invariants_H.thy
@@ -996,6 +996,7 @@ definition max_armKSGICVCPUNumListRegs :: nat where
 definition valid_arch_state' :: "kernel_state \<Rightarrow> bool" where
   "valid_arch_state' \<equiv> \<lambda>s.
    valid_asid_table' (armKSASIDTable (ksArchState s)) \<and>
+   0 \<notin> ran (armKSVMIDTable (ksArchState s)) \<and>
    (case armHSCurVCPU (ksArchState s) of
       Some (v, b) \<Rightarrow> ko_wp_at' (is_vcpu' and hyp_live') v s
       | _ \<Rightarrow> True) \<and>
